cambio nombres Maps

src/tree/layer1/OrderedMap.dfy
@@ -1,41 +1,19 @@
-type K = int
-type V = int
-type pairKV = (K,V)
+include "../../../src/tree/layer1/UnorderedMap.dfy"
+include "../../../src/tree/layer1/OrderedSetUtils.dfy"
 
-function key(p:pairKV):K
-{p.0}
 
-function value(p:pairKV):V
-{p.1}
 
-/*function Keys(m:map<K,V>): set<K>
-     ensures Keys(m)==set k | k in m :: k
-    // ensures |Keys(m)|==|m|
-     {set k | k in m :: k}
 
-  function Pairs(m : map<K,V> ): set<pairKV>
-     ensures Pairs(m)== (set k,v | k in m && v == m[k] :: (k,v))
-     ensures forall p, p'| p in Pairs(m) && p' in Pairs(m) && p!=p' :: p.0!=p'.0
-     ensures forall k, v  | k in m && m[k]==v:: (k,v) in Pairs(m)
-     ensures forall k,v | (k,v) in Pairs(m) :: k in m && m[k]==v
-    // ensures |Pairs(m)|==|Keys(m)|
-     { 
-       (set k,v | k in m && v == m[k] :: (k,v))}
-*/
 
-trait MapKeyValueIterator{
 
-function Parent(): MapKeyValue
-    reads this
-
-predicate Valid()
-    reads this, Parent(), Parent().Repr()
+trait OrderedMapIterator extends UnorderedMapIterator{
 
 function Traversed():set<K>
     reads this, Parent(), Parent().Repr()
     requires Valid()
     requires Parent().Valid() 
     ensures Traversed() <= (Parent().Model().Keys)
+    ensures forall x,y | x in Traversed() && y in Parent().Model().Keys-Traversed() :: x < y
 
 function method Peek():pairKV 
     reads this, Parent(), Parent().Repr()
@@ -43,9 +21,13 @@ function method Peek():pairKV
     requires Parent().Valid()
     requires HasNext()
     ensures Peek() in Parent().Model().Items &&
-            key(Peek()) !in Traversed() &&
-            // key(Peek()) in Parent().Model() && 
-            value(Peek())==Parent().Model()[key(Peek())]
+            key(Peek()) !in Traversed() 
+    ensures key(Peek())==elemth(Parent().Model().Keys,|Traversed()|)  &&
+            value(Peek()) == Parent().Model()[key(Peek())]      
+    ensures forall k | k in Traversed() :: k < key(Peek())
+    ensures forall k | k in Parent().Model().Keys-Traversed()-{key(Peek())} :: key(Peek()) < k
+    ensures forall k | k in Parent().Model().Keys-Traversed() :: key(Peek()) <= k
+
   
 
  function method HasNext(): bool
@@ -56,6 +38,14 @@ function method Peek():pairKV
     //|Traversed()| < |Parent().Model()| es necesario para poder verificar con cota |s.Model()|-|it.Traversed()|
     ensures !HasNext() ==> Traversed() == Parent().Model().Keys && |Traversed()| == |Parent().Model().Keys|
   
+  function method Index(): int
+    reads this, Parent(), Parent().Repr()
+    requires Valid()
+    requires Parent().Valid()
+    ensures HasNext() ==> Index()==|Traversed()|==|smaller(Parent().Model().Keys,key(Peek()))|
+    ensures !HasNext() ==> Index()==|Parent().Model()|
+  
+
   method Next() returns (p: pairKV)
     modifies this
     requires Valid()
@@ -75,11 +65,46 @@ function method Peek():pairKV
     ensures Parent().Iterators() == old(Parent().Iterators())
 
     ensures p==old(Peek()) && Traversed() == {old(key(Peek()))}+old(Traversed())
-    
+    ensures |Traversed()|==1+|old(Traversed())|
+    ensures HasNext() ==> key(Peek())==elemth(Parent().Model().Keys,|Traversed()|)//already known
+
     ensures forall it | it in Parent().Iterators() && old(it.Valid()) ::
       it.Valid() && (it != this ==> it.Traversed() == old(it.Traversed()) && (it.HasNext() ==> it.Peek()==old(it.Peek())))
 
-  method Copy() returns (it: MapKeyValueIterator)
+function method HasPrev(): bool//igual que HasNext
+    reads this, Parent(), Parent().Repr()
+    requires Valid()
+    requires Parent().Valid()
+    ensures HasPrev()  <==> Traversed() < Parent().Model().Keys && |Traversed()| < |Parent().Model().Keys|
+    //|Traversed()| < |Parent().Model()| es necesario para poder verificar con cota |s.Model()|-|it.Traversed()|
+    ensures !HasPrev() ==> Traversed() == Parent().Model().Keys && |Traversed()| == |Parent().Model().Keys|
+  
+
+  method Prev() returns (p: pairKV)
+    modifies this
+    requires Valid()
+    requires Parent().Valid()
+    requires HasNext() 
+    requires allocated(Parent())
+    requires forall it | it in Parent().Repr() :: allocated(it)
+    ensures Parent().Valid()
+    ensures Valid()
+    ensures old(Parent()) == Parent()
+    ensures old(Parent().Model()) == Parent().Model()
+
+    ensures forall x {:trigger x in Parent().Repr(), x in old(Parent().Repr())} | x in Parent().Repr() - old(Parent().Repr()) :: fresh(x)
+    ensures fresh(Parent().Repr()-old(Parent().Repr()))
+    ensures forall x | x in Parent().Repr() :: allocated(x)
+
+    ensures Parent().Iterators() == old(Parent().Iterators())
+    ensures p==old(Peek())  
+    ensures old(Traversed())=={} ==> Traversed()==Parent().Model().Keys
+    ensures old(Traversed())!={} ==> (Traversed()==old(Traversed())-{maximum(old(Traversed()))} &&
+                                      (HasNext() ==> key(Peek())==maximum(old(Traversed()))))
+    ensures forall it | it in Parent().Iterators() && old(it.Valid()) ::
+      it.Valid() && (it != this ==> it.Traversed() == old(it.Traversed()) && (it.HasNext() ==> it.Peek()==old(it.Peek())))
+
+  method Copy() returns (it: UnorderedMapIterator)
     modifies Parent(), Parent().Repr()
     requires Valid()
     requires Parent().Valid()
@@ -95,61 +120,50 @@ function method Peek():pairKV
     ensures fresh(Parent().Repr()-old(Parent().Repr()))
     ensures forall x | x in Parent().Repr() :: allocated(x)
     
+    ensures it is OrderedMapIterator
     ensures it.Valid()
     ensures Parent().Iterators() == {it} + old(Parent().Iterators())
     ensures Parent() == it.Parent()
-    ensures Traversed() == it.Traversed() && (it.HasNext() ==> Peek()==it.Peek())
+
+    ensures Traversed() == it.Traversed() 
+    ensures HasNext() ==> Peek()==it.Peek()
     ensures forall it | it in old(Parent().Iterators()) && old(it.Valid()) ::
       it.Valid() && it.Traversed() == old(it.Traversed()) && (it.HasNext() ==> it.Peek()==old(it.Peek()))
 
 
 }
 
-trait MapKeyValue {
+trait OrderedMap extends UnorderedMap {
   
-   function ReprDepth(): nat
-    reads this
-    ensures ReprDepth() > 0
-
-  function ReprFamily(n: nat): set<object>
-    decreases n
-    requires n <= ReprDepth()
-    ensures n > 0 ==> ReprFamily(n) >= ReprFamily(n-1)
-    reads this, if n == 0 then {} else ReprFamily(n-1)
-
-  function Repr(): set<object>
-    reads this, ReprFamily(ReprDepth()-1)
-  {
-    ReprFamily(ReprDepth())
-  }
-
-  lemma UselessLemma()
-    ensures Repr() == ReprFamily(ReprDepth());
-
-  predicate Valid()
-    reads this, Repr()
-
-  function Model(): map<K,V>
-    reads this, Repr()
-    requires Valid()
-
-  
-  function method Empty(): bool
-    reads this, Repr()
-    requires Valid()
-    ensures Empty() <==> Model() == map[]
-  
- function method Size(): nat
-    reads this, Repr()
-    requires Valid()
-    ensures Size() == |Model()|
-
- function Iterators(): set<MapKeyValueIterator>
+ 
+ function Iterators(): set<UnorderedMapIterator>
     reads this, Repr()
     requires Valid()
     ensures forall it | it in Iterators() :: it in Repr() && it.Parent() == this
+    ensures forall it | it in Iterators() :: it is OrderedMapIterator
 
-method First() returns (it: MapKeyValueIterator)
+method First() returns (it: UnorderedMapIterator)
+    modifies this, Repr()
+    requires Valid()
+    requires forall x | x in Repr() :: allocated(x)
+    ensures Valid()
+    ensures Model() == old(Model())
+
+    ensures forall x {:trigger x in Repr(), x in old(Repr())} | x in Repr() - old(Repr()) :: fresh(x)
+    ensures fresh(Repr()-old(Repr()))
+    ensures forall x | x in Repr() :: allocated(x)
+
+    ensures it is OrderedMapIterator
+    ensures fresh(it)
+    ensures Iterators() == {it} + old(Iterators())
+    ensures it.Valid()
+    ensures it.Parent() == this
+    ensures it.Traversed()=={} 
+    ensures Model()!=map[] ==> it.HasNext() && key(it.Peek())==elemth(Model().Keys,0)
+    ensures forall it | it in old(Iterators()) && old(it.Valid()) ::
+      it.Valid() && it.Traversed() == old(it.Traversed()) && (it.HasNext() ==> it.Peek()==old(it.Peek()))
+
+  method Last() returns (it: OrderedMapIterator)//iterator to the last element
     modifies this, Repr()
     requires Valid()
     requires forall x | x in Repr() :: allocated(x)
@@ -164,66 +178,22 @@ method First() returns (it: MapKeyValueIterator)
     ensures Iterators() == {it} + old(Iterators())
     ensures it.Valid()
     ensures it.Parent() == this
-    ensures it.Traversed()=={} 
+    ensures Model()!=map[] ==> it.HasNext() && it.Traversed()==Model().Keys-{elemth(Model().Keys,|Model().Keys|-1)} && key(it.Peek())==elemth(Model().Keys,|Model().Keys|-1)
+    ensures Model()==map[] ==> it.Traversed()=={}
     ensures forall it | it in old(Iterators()) && old(it.Valid()) ::
       it.Valid() && it.Traversed() == old(it.Traversed()) && (it.HasNext() ==> it.Peek()==old(it.Peek()))
 
- method count(x:int) returns (c:int)
-    requires Valid()
-    ensures Valid() 
-    ensures if (x in Model()) then c==1 else c==0
-
-method at(k:K) returns (v:V)
-    //modifies this,Repr()
-    requires Valid()
-    requires forall x | x in Repr() :: allocated(x)
-    requires k in Model()
-    ensures Valid()
-    //ensures Model()==old(Model())
-    ensures v == Model()[k] 
-
-    ensures forall x {:trigger x in Repr(), x in old(Repr())} | x in Repr() - old(Repr()) :: fresh(x)
-    ensures fresh(Repr()-old(Repr()))
-    ensures forall x | x in Repr() :: allocated(x)
-   
-    ensures Iterators() == old(Iterators())
-
- method add(k:K,v:V)
-    modifies this,Repr()
-    requires Valid()
-    requires forall x | x in Repr() :: allocated(x)
-    ensures Valid()
-    ensures Model() == old(Model())[k:=v] 
-
-    ensures forall x {:trigger x in Repr(), x in old(Repr())} | x in Repr() - old(Repr()) :: fresh(x)
-    ensures fresh(Repr()-old(Repr()))
-    ensures forall x | x in Repr() :: allocated(x)
-   
-    ensures Iterators() == old(Iterators())
-
-
-method remove(k:int) 
-    modifies this,Repr()
-    requires Valid()
-    requires forall x | x in Repr() :: allocated(x)
-    ensures Valid()
-    ensures Model()== map k' | k' in old(Model()) && k'!=k::old(Model())[k']
-
-    ensures forall x {:trigger x in Repr(), x in old(Repr())} | x in Repr() - old(Repr()) :: fresh(x)
-    ensures fresh(Repr()-old(Repr()))
-    ensures forall x | x in Repr() :: allocated(x)
-
-    ensures Iterators() == old(Iterators())
 
 
 
-method find(k:K) returns (newt:MapKeyValueIterator)
+method find(k:K) returns (newt:UnorderedMapIterator)
     modifies this, Repr()
     requires Valid()
     requires forall x | x in Repr() :: allocated(x)
     ensures Valid() 
     ensures Model()==old(Model())
     
+    ensures newt is OrderedMapIterator
     ensures fresh(newt) 
     ensures newt.Valid() && newt.Parent()==this
     ensures k in old(Model()) ==> newt.HasNext() && key(newt.Peek())==k
@@ -235,7 +205,7 @@ method find(k:K) returns (newt:MapKeyValueIterator)
 
     ensures Iterators() == {newt}+old(Iterators())
 
-  method insert(mid: MapKeyValueIterator, k: K, v : V) returns (newt:MapKeyValueIterator)
+  method insert(mid: UnorderedMapIterator, k: K, v : V) returns (newt:UnorderedMapIterator)
     modifies this, Repr()
     requires Valid()
     requires mid.Valid() 
@@ -245,10 +215,11 @@ method find(k:K) returns (newt:MapKeyValueIterator)
     ensures Valid()
     ensures Model() == old(Model())[k:=v]
 
+    ensures newt is OrderedMapIterator
     ensures fresh(newt)
     ensures Iterators() == {newt}+old(Iterators())
     ensures newt.Valid() && newt.Parent()==this  
-    ensures newt.HasNext() && newt.Peek()==(k,v)
+    ensures newt.HasNext() && newt.Peek()==(k,v) && newt.Traversed()==smaller(Model().Keys,k)
 
     ensures forall x {:trigger x in Repr(), x in old(Repr())} | x in Repr() - old(Repr()) :: fresh(x)
     ensures fresh(Repr()-old(Repr()))
@@ -259,7 +230,7 @@ method find(k:K) returns (newt:MapKeyValueIterator)
 
 
 
-  method erase(mid:MapKeyValueIterator) returns (next: MapKeyValueIterator)
+  method erase(mid:UnorderedMapIterator) returns (next: UnorderedMapIterator)
     modifies this, Repr()
     requires Valid()
     requires mid.Valid()
@@ -269,69 +240,17 @@ method find(k:K) returns (newt:MapKeyValueIterator)
     requires forall x | x in Repr() :: allocated(x)
     ensures Valid()
     ensures Model()== map k | k in old(Model()) && k!=old(key(mid.Peek()))::old(Model())[k]
-    ensures |Model()|==|old(Model())|-1
-
+    
+    ensures next is OrderedMapIterator
     ensures fresh(next)
     ensures Iterators() == {next}+old(Iterators())
     ensures next.Valid() && next.Parent()==this 
-    ensures next.Traversed()==old(mid.Traversed()) 
+    ensures next.Traversed()==old(mid.Traversed()) &&
+                (next.HasNext() ==> key(next.Peek())==elemth(Model().Keys,|next.Traversed()|) && value(next.Peek())==Model()[key(next.Peek())])
+
 
     ensures forall x {:trigger x in Repr(), x in old(Repr())} | x in Repr() - old(Repr()) :: fresh(x)
     ensures fresh(Repr()-old(Repr()))
     ensures forall x | x in Repr() :: allocated(x)
  
-}
-
-lemma prove(m:map<K,V>)
-ensures forall k | k in m.Keys :: m[k] in m.Values
-ensures forall p | p in m.Items:: key(p) in m && value(p)==m[key(p)]
-ensures |m|==|m.Keys|
-{}
-
-
-method {:verify true} main(s:MapKeyValue)
-modifies s, s.Repr()
-requires s.Valid() && s.Empty()
-requires forall x | x in s.Repr() :: allocated(x)
-ensures s.Valid()
-ensures forall x {:trigger x in s.Repr(), x in old(s.Repr())} | x in s.Repr() - old(s.Repr()) :: fresh(x)
-ensures fresh(s.Repr()-old(s.Repr()))
-ensures forall x | x in s.Repr() :: allocated(x)
-{
-  assert s.Model()==map[];
- s.add(1,2);
- var x:= s.at(1);
- assert s.Model()==map[1:=2];
- s.add(1,3);
- x:=s.at(1);
- assert x==3;
-
- var z:=s.count(1);
- assert z==1;
- z:=s.count(7);
- assert z==0;
- s.add(2,3); s.add(3,4); s.add(4,5);
-
- var it:=s.First();
- var cont:=0; 
-  while (it.HasNext())
-     decreases |s.Model()|
-    //decreases |s.Model()-it.Model().0|
-    //decreases s.Model()-it.Traversed()
-     invariant s.Valid() 
-     invariant it.Valid() && it in s.Iterators() && it.Parent()==s  
-     invariant  forall x {:trigger x in s.Repr(), x in old(s.Repr())} | x in s.Repr() - old(s.Repr()) :: fresh(x)
-     invariant fresh(s.Repr()-old(s.Repr()))
-     invariant forall x | x in s.Repr() :: allocated(x)
-    {
-     it:=s.erase(it);
-
-    } 
-   assert it.Traversed()==s.Model().Keys; 
-
-   s.remove(1);
-    z:=s.count(1);
- assert z==0;
-
-
 }
